new proofs by KY

src/InferWidth_new.v
@@ -46,55 +46,55 @@ Definition make_vx_implicit (v : vertex_type) : vertex_type :=
     | Node gt => Node (fgtyp_add_implicit gt)
     end.
 
-Fixpoint make_gtyp_implicit (vm : CEP.t vertex_type) (tl : seq (ProdVarOrder.t * fgtyp * HiF.forient)) : option (CEP.t vertex_type) := 
+Fixpoint make_gtyp_implicit (vm nvm : CEP.t vertex_type) (tl : seq (ProdVarOrder.t * fgtyp * HiF.forient)) : option (CEP.t vertex_type) := 
 match tl with
     | nil => Some vm
-    | (pv, gt, _) :: tl => if not_implicit gt then make_gtyp_implicit vm tl
-                         else match CEP.find pv vm with
-                             | Some vx => let vm' := CEP.add pv (make_vx_implicit vx) vm in make_gtyp_implicit vm' tl
-                             | None => None
-                             end
+    | (pv, gt, _) :: tl => match CEP.find pv vm with
+                          | Some vx => let vm' := (if not_implicit gt then CEP.add pv vx nvm
+                                        else CEP.add pv (make_vx_implicit vx) nvm) in make_gtyp_implicit vm vm' tl
+                          | None => None
+                          end
     end.
 
-Definition make_p_implicit (vm : CEP.t vertex_type) (p : HiFP.hfport) : option (CEP.t vertex_type) :=
+Definition make_p_implicit (vm nvm : CEP.t vertex_type) (p : HiFP.hfport) : option (CEP.t vertex_type) :=
    match p with
    | Finput v t => let tl := list_gtypref v t HiF.Source in
-                   make_gtyp_implicit vm tl
+                   make_gtyp_implicit vm nvm tl
    | Foutput v t => let tl := list_gtypref v t HiF.Sink in
-                   make_gtyp_implicit vm tl
+                   make_gtyp_implicit vm nvm tl
    end.
 
-Fixpoint  make_ps_implicit (vm : CEP.t vertex_type) (ps : seq HiFP.hfport) : option (CEP.t vertex_type) :=
+Fixpoint  make_ps_implicit (vm nvm : CEP.t vertex_type) (ps : seq HiFP.hfport) : option (CEP.t vertex_type) :=
     match ps with
-    | nil => Some vm
-    | hd :: tl => match make_p_implicit vm hd with
-                | Some vm' => make_ps_implicit vm' tl
+    | nil => Some nvm
+    | hd :: tl => match make_p_implicit vm nvm hd with
+                | Some vm' => make_ps_implicit vm vm' tl
                 | None => None
                 end
     end.
 
-Fixpoint make_s_implicit (vm : CEP.t vertex_type) (st : HiFP.hfstmt) : option (CEP.t vertex_type) :=
+Fixpoint make_s_implicit (vm nvm : CEP.t vertex_type) (st : HiFP.hfstmt) : option (CEP.t vertex_type) :=
 (* change the vertex of statement st in vm to implicit-width if st defines an implicit-width component *)
    match st with
-  | Sskip => Some vm
+  | Sskip => Some nvm
   | Swire v t => let tl := list_gtypref v t HiF.Duplex in
-                 make_gtyp_implicit vm tl
+                 make_gtyp_implicit vm nvm tl
   | Sreg v r => let tl := list_gtypref v (type r) HiF.Duplex in
-                make_gtyp_implicit vm tl
+                make_gtyp_implicit vm nvm tl
   | Smem v m => (*TBD*) Some vm
   | Sinst v inst => (*TBD*) Some vm
-  | Swhen _ s1 s2 => match make_ss_implicit vm s1 with
-                    | Some vm' => make_ss_implicit vm s2
+  | Swhen _ s1 s2 => match make_ss_implicit vm nvm s1 with
+                    | Some vm' => make_ss_implicit vm nvm s2
                     | None => None
                     end
-  | _ => Some vm 
+  | _ => Some nvm 
   end
-with make_ss_implicit (vm : CEP.t vertex_type) (ss : HiFP.hfstmt_seq) : option (CEP.t vertex_type) :=
+with make_ss_implicit (vm nvm : CEP.t vertex_type) (ss : HiFP.hfstmt_seq) : option (CEP.t vertex_type) :=
 (* change the vertices of statements ss in vm to implicit-width if ss defines implicit-width components *)
    match ss with
-  | Qnil => Some vm
-  | Qcons s st => match make_s_implicit vm s with
-                | Some vm' => make_ss_implicit vm st
+  | Qnil => Some nvm
+  | Qcons s st => match make_s_implicit vm nvm s with
+                | Some vm' => make_ss_implicit vm vm' st
                 | None => None
                 end
   end.
@@ -102,11 +102,11 @@ with make_ss_implicit (vm : CEP.t vertex_type) (ss : HiFP.hfstmt_seq) : option (
 Definition make_vm_implicit (F : HiFP.hfmodule) (vm : CEP.t vertex_type) : option (CEP.t vertex_type) :=
    (* in vm, change the type of vertex (explicit to implicit) according to its declaration in F. *)
    match F with
-   | FInmod _ pp ss => match make_ps_implicit vm pp with
-                      | Some vm' => make_ss_implicit vm' ss
+   | FInmod _ pp ss => match make_ps_implicit vm (CEP.empty vertex_type) pp with
+                      | Some vm' => make_ss_implicit vm vm' ss
                       | None => None
                       end
-   | FExmod _ _ _ => Some vm
+   | FExmod _ _ _ => Some (CEP.empty vertex_type)
    end.
 
 Fixpoint ft_find_sub (checkt : ftype) (num : N) (ori : HiF.forient) : option (ftype * HiF.forient) :=
@@ -486,9 +486,12 @@ Fixpoint check_connect_non_passive_type (t_tgt t_src : seq (ProdVarOrder.T * fgt
   match t_tgt, t_src with
   | nil, nil => true
   | (_, thd, HiF.Sink) :: ttl, (_, shd, HiF.Source) :: stl 
-  | (_, thd, HiF.Sink) :: ttl, (_, shd, HiF.Duplex) :: stl => connect_fgtyp_compatible thd shd && check_connect_non_passive_type ttl stl
+  | (_, thd, HiF.Sink) :: ttl, (_, shd, HiF.Duplex) :: stl 
+  | (_, thd, HiF.Duplex) :: ttl, (_, shd, HiF.Duplex) :: stl 
+  | (_, thd, HiF.Duplex) :: ttl, (_, shd, HiF.Source) :: stl => connect_fgtyp_compatible thd shd && check_connect_non_passive_type ttl stl
   | (_, thd, HiF.Source) :: ttl, (_, shd, HiF.Sink) :: stl 
-  | (_, thd, HiF.Source) :: ttl, (_, shd, HiF.Duplex) :: stl => connect_fgtyp_compatible shd thd && check_connect_non_passive_type ttl stl
+  | (_, thd, HiF.Source) :: ttl, (_, shd, HiF.Duplex) :: stl 
+  | (_, thd, HiF.Duplex) :: ttl, (_, shd, HiF.Sink) :: stl => connect_fgtyp_compatible shd thd && check_connect_non_passive_type ttl stl
   | _, _ => false
   end.
 
@@ -499,31 +502,32 @@ Fixpoint check_connect_type (t_tgt t_src : seq (ProdVarOrder.T * fgtyp * HiF.for
   | _, _ => false
   end.
 
-Definition connect_non_passive_type (t_tgt t_src : ftype) (ori_tgt ori_src : HiF.forient) : Prop :=
-  ftype_equiv t_tgt t_src && check_connect_non_passive_type (list_gtypref (N0, N0) t_tgt ori_tgt) (list_gtypref (N0, N0) t_src ori_src). 
+Definition connect_non_passive_type (ref_tgt ref_src : ProdVarOrder.T) (t_tgt t_src : ftype) (ori_tgt ori_src : HiF.forient) : Prop :=
+  ftype_equiv t_tgt t_src && check_connect_non_passive_type (list_gtypref ref_tgt t_tgt ori_tgt) (list_gtypref ref_src t_src ori_src). 
 
-Definition connect_type (t_tgt t_src : ftype) (ori_tgt ori_src : HiF.forient) : Prop :=
-  ftype_equiv t_tgt t_src && check_connect_type (list_gtypref (N0, N0) t_tgt ori_tgt) (list_gtypref (N0, N0) t_src ori_src).
+Definition connect_type (ref : ProdVarOrder.T) (t_tgt t_src : ftype) (ori_tgt ori_src : HiF.forient) : Prop :=
+  ftype_equiv t_tgt t_src && check_connect_type (list_gtypref ref t_tgt ori_tgt) (list_gtypref (N0, N0) t_src ori_src).
 
-Fixpoint Sem_frag_stmt (vm_old : CEP.t vertex_type) (ct_old : CEP.t def_expr) (s : HiFP.hfstmt) (vm_new : CEP.t vertex_type) (ct_new : CEP.t def_expr) (tmap : CEP.t (ftype * HiF.forient)) : Prop :=
+Fixpoint Sem_frag_stmt (vm_old : CEP.t vertex_type) (s : HiFP.hfstmt) (vm_new : CEP.t vertex_type) (tmap : CEP.t (ftype * HiF.forient)) : Prop :=
    (* The predicate returns True if vm_new/ct_new can be constructed from vm_old/ct_old by applying s.
    type checking, constraints *)
    match s with
-   | Sskip => CEP.Equal vm_old vm_new /\ CEP.Equal ct_old ct_new
+   | Sskip => CEP.Equal vm_old vm_new 
    | Sfcnct (Eid ref_tgt) (Eref (Eid ref_src)) => (* allow non-passive types *)
           match type_of_ref ref_tgt tmap, type_of_ref ref_src tmap with
-          | Some (ft_tgt, ori_tgt), Some (ft_src, ori_src) => connect_non_passive_type ft_tgt ft_src ori_tgt ori_src
+          | Some (ft_tgt, ori_tgt), Some (ft_src, ori_src) => connect_non_passive_type ref_tgt ref_src ft_tgt ft_src ori_tgt ori_src
           | _, _ => False
           end
+   | Sfcnct (Eid ref_tgt) (Eref _) => False
    | Sfcnct (Eid ref) expr =>
           match type_of_ref ref tmap, type_of_expr expr tmap with
-          | Some (ft_tgt, ori_tgt), Some (exist ft_src _) => connect_type ft_tgt ft_src ori_tgt HiF.Source
+          | Some (ft_tgt, ori_tgt), Some (exist ft_src _) => connect_type ref ft_tgt ft_src ori_tgt HiF.Source
           | _, _ => False
           end
    | Sreg v reg =>
        match reset reg with
         | Rst _ rst_val => match CEP.find v tmap, type_of_expr rst_val tmap with
-            | Some (newft, _), Some (exist rst_val_type _) => connect_type newft rst_val_type HiF.Duplex HiF.Duplex
+            | Some (newft, _), Some (exist rst_val_type _) => connect_type v newft rst_val_type HiF.Duplex HiF.Duplex
             | _, _ => false
             end
         | NRst => True (* type check newft: we only need to verify newft is passive *)
@@ -532,28 +536,28 @@ Fixpoint Sem_frag_stmt (vm_old : CEP.t vertex_type) (ct_old : CEP.t def_expr) (s
    | Sinst var1 var2 => False (* ? *)
    | Swhen cond ss_true ss_false =>
        if type_of_expr cond tmap is Some (exist (Gtyp (Fuint 1)) _)
-       then exists (vm_true : CEP.t vertex_type) (ct_true ct_false : CEP.t def_expr),
-                   Sem_frag_stmts vm_old ct_old ss_true vm_true ct_true tmap
+       then exists (vm_true : CEP.t vertex_type),
+                   Sem_frag_stmts vm_old ss_true vm_true tmap
                 /\
-                   Sem_frag_stmts vm_true (extend_map_with ct_old ct_true) ss_false vm_new ct_false tmap
+                   Sem_frag_stmts vm_true ss_false vm_new tmap
        else False
    | Sinvalid _
    | Swire _ _
    | Snode _ _ => True
    | _ => False
    end
-with Sem_frag_stmts (vm_old : CEP.t vertex_type) (ct_old : CEP.t def_expr) (ss : HiFP.hfstmt_seq) (vm_new : CEP.t vertex_type) (ct_new : CEP.t def_expr) (tmap : CEP.t (ftype * HiF.forient)) : Prop :=
+with Sem_frag_stmts (vm_old : CEP.t vertex_type) (ss : HiFP.hfstmt_seq) (vm_new : CEP.t vertex_type) (tmap : CEP.t (ftype * HiF.forient)) : Prop :=
 match ss with
 | Qnil =>
        CEP.Equal vm_old vm_new
 | Qcons s ss' =>
-    exists (vm' : CEP.t vertex_type) (ct' : CEP.t def_expr),
-           Sem_frag_stmt vm_old ct_old s vm' ct' tmap
+    exists (vm' : CEP.t vertex_type),
+           Sem_frag_stmt vm_old s vm' tmap
         /\
-           Sem_frag_stmts vm' ct' ss' vm_new ct_new tmap
+           Sem_frag_stmts vm' ss' vm_new tmap
 end.
 
-Definition Sem (F : HiFP.hfmodule) (vm : CEP.t vertex_type) (ct : CEP.t def_expr) : Prop :=
+Definition Sem (F : HiFP.hfmodule) (vm : CEP.t vertex_type) : Prop :=
 (* The predicate returns True if G = (vm, ct) conforms to F.
    (If F has errors, there is no such G.)
    (If F has implicit width components, then there are many such Gs.)
@@ -569,7 +573,7 @@ match F with
                                  (CEP.empty def_expr)
                                  pp vm' ct' tmap
                /\
-                  Sem_frag_stmts vm' ct' ss vm ct tmap)
+                  Sem_frag_stmts vm' ss vm tmap)
     | None => False
     end
 | FExmod _ _ _ => False
@@ -603,12 +607,15 @@ Fixpoint add_expr_connect_non_passive (el1 el2 : seq (ProdVarOrder.t * fgtyp * H
   match el1, el2 with
   | nil, nil => Some var2exprs
   | (ref1, _, HiF.Sink) :: tl1, (ref2, _, HiF.Source) :: tl2 
+  | (ref1, _, HiF.Sink) :: tl1, (ref2, _, HiF.Duplex) :: tl2 
+  | (ref1, _, HiF.Duplex) :: tl1, (ref2, _, HiF.Duplex) :: tl2 
   | (ref1, _, HiF.Duplex) :: tl1, (ref2, _, HiF.Source) :: tl2 => 
                 match CEP.find ref1 var2exprs with
                 | Some ls => add_expr_connect_non_passive tl1 tl2 (CEP.add ref1 ((Eref (Eid ref2)) :: ls) var2exprs)
                 | None => add_expr_connect_non_passive tl1 tl2 (CEP.add ref1 [::(Eref (Eid ref2))] var2exprs)
                 end
   | (ref1, _, HiF.Source) :: tl1, (ref2, _, HiF.Sink) :: tl2 
+  | (ref1, _, HiF.Duplex) :: tl1, (ref2, _, HiF.Sink) :: tl2 
   | (ref1, _, HiF.Source) :: tl1, (ref2, _, HiF.Duplex) :: tl2 => 
                 match CEP.find ref2 var2exprs with
                 | Some ls => add_expr_connect_non_passive tl1 tl2 (CEP.add ref2 ((Eref (Eid ref1)) :: ls) var2exprs)
@@ -1018,13 +1025,440 @@ Definition InferWidths_m F : option (HiFP.hfmodule * CEP.t (ftype * HiF.forient)
   | None => None
   end.
 
+Lemma check_connect_type_correct : forall ft te, (forall n,
+  match nth_error ft n, nth_error te n with
+  | Some (_, gt, _), Some (_, gte, _) => connect_fgtyp_compatible gt gte
+  | None, None => true
+  | _, _ => false
+  end) -> check_connect_type ft te.
+Proof.
+Admitted.
+
+Lemma check_connect_non_passive_type_correct : forall ft te, (forall n, 
+  match nth_error ft n, nth_error te n with
+  | Some (_, thd, HiF.Sink), Some (_, shd, HiF.Source)
+  | Some (_, thd, HiF.Sink), Some (_, shd, HiF.Duplex)
+  | Some (_, thd, HiF.Duplex), Some (_, shd, HiF.Duplex)
+  | Some (_, thd, HiF.Duplex), Some (_, shd, HiF.Source) => connect_fgtyp_compatible thd shd
+  | Some (_, thd, HiF.Source), Some (_, shd, HiF.Sink)
+  | Some (_, thd, HiF.Source), Some (_, shd, HiF.Duplex)
+  | Some (_, thd, HiF.Duplex), Some (_, shd, HiF.Sink)=> connect_fgtyp_compatible shd thd
+  | None, None => true
+  |  _, _ => false
+  end) -> check_connect_non_passive_type ft te.
+Proof.
+Admitted.
+
+Lemma listgtyp_eq t_tgt t_expr : forall n ref0 ref1 ori0 ori1 ori2 ori3 pv0 pv1 gt gte, ftype_equiv t_tgt t_expr -> nth_error (list_gtypref ref0 t_tgt ori0) n =
+  Some (pv0, gt, ori2) -> nth_error (list_gtypref ref1 t_expr ori1) n = Some (pv1, gte, ori3) -> fgtyp_equiv gt gte.
+Proof.
+Admitted.
+
+Lemma infer_cons_order : forall order1 order2 var2exprs tmap tmap' newtm, InferWidths_fun (order1 ++ order2) var2exprs tmap = Some newtm -> InferWidths_fun order1 var2exprs tmap = Some tmap' ->
+  InferWidths_fun order2 var2exprs tmap' = Some newtm.
+Proof.
+Admitted.
+
+Lemma split_expr_type_correct : forall expr rhs_expr_ls t_expr newtm (p : ftype_not_implicit_width t_expr), type_of_expr expr newtm = Some (exist ftype_not_implicit_width t_expr p) -> list_gtypexpr expr t_expr = Some rhs_expr_ls ->
+  forall n, match nth_error (list_gtypref (0%num, 0%num) t_expr HiF.Source) n, nth_error rhs_expr_ls n with
+            | Some (_, gt, _), Some texpr => exists p0, type_of_expr texpr newtm = Some (exist ftype_not_implicit_width (Gtyp gt) p0)
+            | _, _ => true
+            end.
+Proof.
+Admitted.
+
+Lemma InferWidth_fun_correct : forall pv el tmap newtm, InferWidth_fun pv el tmap = Some newtm -> forall expr, expr \in el -> 
+      match CEP.find (fst pv, N0) newtm with
+      | Some (checkt, ori) => match ft_find_sub checkt pv.2 ori, type_of_expr expr newtm with
+                              | Some (Gtyp nt, _), Some (exist (Gtyp te) p) => fgtyp_equiv nt te -> connect_fgtyp_compatible nt te
+                              | _,_ => true
+                              end
+      | _ => true
+      end.
+Proof.
+Admitted.
+
+Lemma list_fsteq : forall ref_tgt tgt v_tgt ori, In v_tgt (list_gtypref ref_tgt tgt ori) -> ref_tgt.1 = v_tgt.1.1.1.
+Proof.
+Admitted.
+
+Lemma list_typeq ref_tgt : forall tmap t_tgt ori n pv0 gt ori0, type_of_ref ref_tgt tmap = Some (t_tgt, ori) -> nth_error (list_gtypref ref_tgt t_tgt ori) n = Some (pv0, gt, ori0) -> type_of_ref pv0 tmap = Some (Gtyp gt, ori).
+Proof.
+Admitted.
+
+Lemma infernotin_eq : forall pv inferorder var2exprs tmap newtm, pv \notin inferorder -> InferWidths_fun inferorder var2exprs tmap = Some newtm ->
+type_of_ref pv newtm = type_of_ref pv tmap /\ (match CEP.find pv var2exprs with
+                                              | Some el => forall e, e \in el -> type_of_expr e newtm = type_of_expr e tmap
+                                              |  _ => true
+                                              end). 
+Proof.
+Admitted.
+
+Lemma preexpr_in: forall ps ss tmap newtm var2exprs ref_tgt t_tgt ori expr texpr t_expr rhs_expr_ls pe n pv0 gt ori0 el, ports_stmts_tmap' ps ss = Some (tmap, var2exprs) -> Qin (Sfcnct (Eid ref_tgt) expr) ss -> type_of_ref ref_tgt newtm = Some (t_tgt, ori) ->
+type_of_expr expr newtm = Some (exist ftype_not_implicit_width t_expr pe) -> list_gtypexpr expr t_expr = Some rhs_expr_ls -> nth_error rhs_expr_ls n = Some texpr -> CEP.find pv0 var2exprs = Some el -> 
+nth_error (list_gtypref ref_tgt t_tgt ori) n = Some (pv0, gt, ori0) -> texpr \in el.
+Proof.
+Admitted.
+
+Lemma InferWidths_fun_correct : forall pp ss (inferorder : seq ProdVarOrder.t) (var2exprs : CEP.t (seq HiFP.hfexpr)) (tmap0 newtm : CEP.t (ftype * HiF.forient)),
+  InferWidths_fun inferorder var2exprs tmap0 = Some newtm -> ports_stmts_tmap' pp ss = Some (tmap0, var2exprs) -> 
+  (forall (hfs : HiFP.hfstmt), Qin hfs ss -> match hfs with
+    | Sfcnct (Eid ref_tgt) (Eref (Eid ref_src)) => match type_of_ref ref_tgt newtm, type_of_ref ref_src newtm with
+                                      | Some (t_tgt, ori_tgt), Some (t_src, ori_src) => ftype_equiv t_tgt t_src -> connect_non_passive_type ref_tgt ref_src t_tgt t_src ori_tgt ori_src
+                                      | _, _ => True
+                                      end 
+    | Sfcnct (Eid ref_tgt) (Eref _) => True
+    | Sfcnct (Eid ref_tgt) expr_src => match type_of_ref ref_tgt newtm, type_of_expr expr_src newtm with
+                                      | Some (t_tgt, ori), Some (exist t_expr _) => ftype_equiv t_tgt t_expr -> connect_type ref_tgt t_tgt t_expr ori HiF.Source
+                                      | _, _ => True
+                                      end
+    | _ => True
+    end).
+Proof.
+  intros ps ss inferorder var2exprs tmap newtm Hinfer Hpre hfs Hin.
+  case Hs : hfs => [||||||ref expr||]; try done.
+  case He : expr => [ct c| c e1 | u e1 | op e1 e2 | c e1 e2 | c e1 | ref0 ]; try done. 
+  (* const *)
+  1,2,3,4,5,6 : rewrite -He; clear He; rewrite Hs in Hin; clear Hs hfs;
+                case Href : ref => [ref_tgt|||]; try done;
+                case Htr : (type_of_ref ref_tgt newtm) => [[t_tgt ori]|]; try done;
+                case Hte : (type_of_expr expr newtm) => [[t_expr pe]|] ; try done; intro Heq;
+                rewrite /connect_type;
+                apply rwP with (P := ftype_equiv t_tgt t_expr /\
+    check_connect_type (list_gtypref ref_tgt t_tgt ori)
+    (list_gtypref (0%num, 0%num) t_expr HiF.Source)).
+  1,3,5,7,9,11 : apply andP.
+  1,2,3,4,5,6 : split. 
+  1,3,5,7,9,11 : apply Heq. (* hypo *)
+  apply check_connect_type_correct with (ft := list_gtypref ref_tgt t_tgt ori) (te := list_gtypref (0%num, 0%num) t_expr HiF.Source).
+  intros n.
+  case Hlhs : (nth_error (list_gtypref ref_tgt t_tgt ori) n) => [[[pv0 gt] ori0]|].
+  case Hrhs : (nth_error (list_gtypref (0%num, 0%num) t_expr HiF.Source) n) => [[[pv1 gte] ori1]|]; try done.
+  rewrite /connect_fgtyp_compatible.
+  apply rwP with (P := fgtyp_equiv gt gte /\
+    (if not_implicit gt
+    then true
+    else sizeof_fgtyp gte <= sizeof_fgtyp gt)).
+  apply andP.
+  split. 
+  move : Heq Hlhs Hrhs; apply listgtyp_eq.
+  case Himpli : (not_implicit gt); try done.
+
+  assert (exists order1 order2, (inferorder = order1 ++ (pv0 :: order2)) /\ (pv0 \notin order1) 
+    /\ (pv0 \notin order2)).
+  admit. (* inferorder 的正确性，是展开时的标号 *)
+  move : H => [order1 [order2 [H [Horder1 Horder2]]]].
+  generalize Hinfer; rewrite H in Hinfer; move => Hinfer'.
+  case Hinfer1 : (InferWidths_fun order1 var2exprs tmap) => [tmap'|].
+  assert (Hinfer2 : InferWidths_fun (pv0 :: order2) var2exprs tmap' = Some newtm).
+  move : Hinfer Hinfer1.
+  apply infer_cons_order.
+  clear Hinfer.
+  simpl in Hinfer2.
+  case Hel : (CEP.find pv0 var2exprs) => [el|]; rewrite Hel in Hinfer2; try done.
+  case Hinfer : (InferWidth_fun pv0 el tmap') => [newtm'|]; rewrite Hinfer in Hinfer2; try discriminate.
+  case Hsplit : (list_gtypexpr expr t_expr) => [rhs_expr_ls|].
+  generalize Hte; apply split_expr_type_correct with (rhs_expr_ls := rhs_expr_ls) (n := n) in Hte; try done; rewrite Hrhs in Hte; intro Hte'.
+  case Htexpr : (nth_error rhs_expr_ls n) => [texpr|]; rewrite Htexpr in Hte. destruct Hte as [p0 Hte].
+  apply InferWidth_fun_correct with (pv := pv0) (el := el) (tmap := tmap') (newtm := newtm') (expr := texpr) in Hinfer; try done.
+  generalize Htr; rewrite /type_of_ref in Htr; case Hcheckt : (CEP.find (ref_tgt.1, 0%num) newtm) => [[checkt ori_c]|]; rewrite Hcheckt in Htr; try discriminate; intro Htr'.
+  generalize Hlhs; apply nth_error_In in Hlhs; apply list_fsteq in Hlhs; simpl in Hlhs.
+  intro Hlhs'; generalize Hlhs'; apply list_typeq with (tmap := newtm) in Hlhs'; try done.
+  intro Hlhs0; rewrite /type_of_ref -Hlhs in Hlhs'. rewrite -Hlhs in Hinfer.
+  assert (exists checkt' ori_c', CEP.find (ref_tgt.1, 0%num) newtm' = Some (checkt', ori_c')).
+  admit. (* 由 Hcheckt *)
+  destruct H0 as [checkt' [ori_c' Htgt0]]; rewrite Htgt0 in Hinfer.
+  assert (exists nt ori', ft_find_sub checkt' pv0.2 ori_c' = Some (nt, ori')).
+  admit. (* 由 Htr *)
+  destruct H0 as [nt [ori' Hsub0]]; rewrite Hsub0 in Hinfer; rewrite Hcheckt in Hlhs'.
+  apply infernotin_eq with (var2exprs := var2exprs) (tmap := newtm') (newtm := newtm) in Horder2; try done; move : Horder2 => [Horder2 Horder2'].
+  rewrite /type_of_ref -Hlhs Htgt0 Hcheckt in Horder2; rewrite Horder2 in Hlhs'; rewrite Hlhs' in Hsub0; inversion Hsub0; clear Hsub0.
+  rewrite -H1 in Hinfer; clear H1 nt H2 ori'.
+  assert (texpr \in el).
+  rewrite Href in Hin; move : Hpre Hin Htr' Hte' Hsplit Htexpr Hel Hlhs0.
+  apply preexpr_in.
+  rewrite Hel in Horder2'; specialize Horder2' with (e := texpr); apply Horder2' in H0; rewrite -H0 Hte in Hinfer; clear Horder2' H0.
+  assert (fgtyp_equiv gt gte).
+  move : Heq Hlhs0 Hrhs; apply listgtyp_eq.
+  apply Hinfer in H0; clear Hinfer; rewrite /connect_fgtyp_compatible in H0.
+  move /andP : H0 => [_ H0]; rewrite Himpli in H0; done.
+  rewrite Href in Hin; move : Hpre Hin Htr Hte' Hsplit Htexpr Hel Hlhs.
+  apply preexpr_in.
+  admit. (* 不是None *)
+  admit. (* 不是None *)
+  admit. (* 不是None *)
+  admit. (* 不是None *)
+  admit. (* 不是None *)
+
+  admit.
+  admit.
+  admit.
+  admit.
+  admit. (* 5个相同case *)
+
+  (* non_passive *)
+  rewrite He in Hs; clear He expr; rewrite Hs in Hin; clear Hs hfs.
+  case Href : ref => [ref_tgt|||]; rewrite Href in Hin; try done.
+  case Href0 : ref0 => [ref_src|||]; rewrite Href0 in Hin; clear Href; try done.
+  case Htgt : (type_of_ref ref_tgt newtm) => [[t_tgt ori_tgt]|]; clear Href0 ref ref0; try done.
+  case Hsrc : (type_of_ref ref_src newtm) => [[t_src ori_src]|]; try done; intro Heq.
+  rewrite /connect_non_passive_type.
+  apply rwP with (P := ftype_equiv t_tgt t_src /\ check_connect_non_passive_type (list_gtypref ref_tgt t_tgt ori_tgt) (list_gtypref ref_src t_src ori_src)).
+  apply andP.
+  split; try done. 
+  apply check_connect_non_passive_type_correct.
+  intro n.
+
+  case Hlhs : (nth_error (list_gtypref ref_tgt t_tgt ori_tgt) n) => [[[pv_tgt gt_tgt] ori_tgt0]|].
+  case Hrhs : (nth_error (list_gtypref ref_src t_src ori_src) n) => [[[pv_src gt_src] ori_src0]|].
+  case Hori_tgt : ori_tgt0.
+  (*rewrite /connect_fgtyp_compatible.
+  apply rwP with (P := fgtyp_equiv gt gte /\
+    (if not_implicit gt
+    then true
+    else sizeof_fgtyp gte <= sizeof_fgtyp gt)).
+  apply andP.
+  split. 
+  move : Heq Hlhs Hrhs; apply listgtyp_eq.
+  case Himpli : (not_implicit gt); try done.*)
+  - (* tgt : source *)
+  assert (exists order1 order2, (inferorder = order1 ++ (pv0 :: order2)) /\ (pv0 \notin order1) 
+    /\ (pv0 \notin order2)).
+  admit. (* inferorder 的正确性，是展开时的标号 *)
+  move : H => [order1 [order2 [H [Horder1 Horder2]]]].
+  generalize Hinfer; rewrite H in Hinfer; move => Hinfer'.
+  case Hinfer1 : (InferWidths_fun order1 var2exprs tmap) => [tmap'|].
+  assert (Hinfer2 : InferWidths_fun (pv0 :: order2) var2exprs tmap' = Some newtm).
+  move : Hinfer Hinfer1.
+  apply infer_cons_order.
+  clear Hinfer.
+  simpl in Hinfer2.
+  case Hel : (CEP.find pv0 var2exprs) => [el|]; rewrite Hel in Hinfer2; try done.
+  case Hinfer : (InferWidth_fun pv0 el tmap') => [newtm'|]; rewrite Hinfer in Hinfer2; try discriminate.
+  case Hsplit : (list_gtypexpr expr t_expr) => [rhs_expr_ls|].
+  generalize Hte; apply split_expr_type_correct with (rhs_expr_ls := rhs_expr_ls) (n := n) in Hte; try done; rewrite Hrhs in Hte; intro Hte'.
+  case Htexpr : (nth_error rhs_expr_ls n) => [texpr|]; rewrite Htexpr in Hte. destruct Hte as [p0 Hte].
+  apply InferWidth_fun_correct with (pv := pv0) (el := el) (tmap := tmap') (newtm := newtm') (expr := texpr) in Hinfer; try done.
+  generalize Htr; rewrite /type_of_ref in Htr; case Hcheckt : (CEP.find (ref_tgt.1, 0%num) newtm) => [[checkt ori_c]|]; rewrite Hcheckt in Htr; try discriminate; intro Htr'.
+  generalize Hlhs; apply nth_error_In in Hlhs; apply list_fsteq in Hlhs; simpl in Hlhs.
+  intro Hlhs'; generalize Hlhs'; apply list_typeq with (tmap := newtm) in Hlhs'; try done.
+  intro Hlhs0; rewrite /type_of_ref -Hlhs in Hlhs'. rewrite -Hlhs in Hinfer.
+  assert (exists checkt' ori_c', CEP.find (ref_tgt.1, 0%num) newtm' = Some (checkt', ori_c')).
+  admit. (* 由 Hcheckt *)
+  destruct H0 as [checkt' [ori_c' Htgt0]]; rewrite Htgt0 in Hinfer.
+  assert (exists nt ori', ft_find_sub checkt' pv0.2 ori_c' = Some (nt, ori')).
+  admit. (* 由 Htr *)
+  destruct H0 as [nt [ori' Hsub0]]; rewrite Hsub0 in Hinfer; rewrite Hcheckt in Hlhs'.
+  apply infernotin_eq with (var2exprs := var2exprs) (tmap := newtm') (newtm := newtm) in Horder2; try done; move : Horder2 => [Horder2 Horder2'].
+  rewrite /type_of_ref -Hlhs Htgt0 Hcheckt in Horder2; rewrite Horder2 in Hlhs'; rewrite Hlhs' in Hsub0; inversion Hsub0; clear Hsub0.
+  rewrite -H1 in Hinfer; clear H1 nt H2 ori'.
+  assert (texpr \in el).
+  rewrite Href in Hin; move : Hpre Hin Htr' Hte' Hsplit Htexpr Hel Hlhs0.
+  apply preexpr_in.
+  rewrite Hel in Horder2'; specialize Horder2' with (e := texpr); apply Horder2' in H0; rewrite -H0 Hte in Hinfer; clear Horder2' H0.
+  assert (fgtyp_equiv gt gte).
+  move : Heq Hlhs0 Hrhs; apply listgtyp_eq.
+  apply Hinfer in H0; clear Hinfer; rewrite /connect_fgtyp_compatible in H0.
+  move /andP : H0 => [_ H0]; rewrite Himpli in H0; done.
+  rewrite Href in Hin; move : Hpre Hin Htr Hte' Hsplit Htexpr Hel Hlhs.
+  apply preexpr_in.
+
+Admitted.
+
+Lemma InferWidths_trans_correct : forall pp ss nps nss newtm vm' vm'' vm (*pv*), (*InferWidths_stage1 (FInmod pv pp ss) = Some newtm ->*) InferWidths_transps pp newtm = Some nps -> InferWidths_transss ss newtm = Some nss ->
+make_ps_implicit vm' (CEP.empty vertex_type) pp = Some vm'' -> make_ss_implicit vm' vm'' ss = Some vm -> ports_stmts_tmap pp ss vm = Some newtm.
+Proof.
+  (*rewrite /ports_stmts_tmap.
+  elim.
+  elim.
+  - simpl; done.
+  - intros s st IH; intros nps nss newtm vm' vm'' vm pv Hinfer Hps Hss Himplips Himpliss.
+    simpl; simpl in Hps; simpl in Hss; simpl in Himplips; simpl in Himpliss.
+    inversion Hps; clear Hps H0 nps; inversion Himplips; rewrite -H0 in Himpliss; clear Himplips H0 vm''.
+    case Htrans : (InferWidths_transs s newtm) => [ns|]; rewrite Htrans in Hss; try discriminate.
+    case Htranss : (InferWidths_transss st newtm) => [nst|]; rewrite Htranss in Hss; try discriminate.
+    case Himplis : (make_s_implicit vm' (CEP.empty vertex_type) s) => [vm0|]; rewrite Himplis in Himpliss; try discriminate.
+    inversion Hss as [Hnss]; clear Hss.
+    case Hss : (stmt_tmap (CEP.empty (ftype * HiF.forient), CEP.empty (ftype * HiF.forient)) s vm) => [tmap_scope'|].
+    case Hsst : (stmts_tmap tmap_scope' st vm) => [[tmap' emap']|].
+    (*apply IH with (nps := [::]) (nss := nst) (newtm := newtm) (pv := pv) in Himpliss; try done.
+
+    case Hsp : (stmt_tmap' (CEP.empty (ftype * HiF.forient)) (CEP.empty (seq HiFP.hfexpr)) s) => [[tmap0 emap0]|]; rewrite Hsp in Hinfer; try discriminate.
+    case Hsps : (stmts_tmap' tmap0 emap0 st) => [[tmap' var2exprs]|]; rewrite Hsps in Hinfer; try discriminate.
+    case Hrl : (lsreg_stmt s) => [rl|]; rewrite Hrl in Hinfer; try discriminate.
+    case Hrls : (lsreg_stmts st) => [rls|]; rewrite Hrls in Hinfer; try discriminate.*)
+    *)
+
+Admitted.
+
 Theorem InferWidths_correct :
-  forall (F : HiFP.hfmodule) (vm' : CEP.t vertex_type) (ct : CEP.t def_expr),
+  forall (F : HiFP.hfmodule) (vm' : CEP.t vertex_type),
     match InferWidths_m F, make_vm_implicit F vm' with
-    | Some (F', _), Some vm => Sem F' vm' ct -> Sem F vm ct
+    | Some (F', _), Some vm => Sem F' vm' -> Sem F vm
     | _, _ => True
     end.
 Proof.
+  intros.
+  case Hinfer : (InferWidths_m F) => [[F' t]|]; try done.
+  case Himplivm : (make_vm_implicit F vm') => [vm|]; try done.
+  rewrite /Sem; rewrite /InferWidths_m in Hinfer.
+  case Hinfer1 : (InferWidths_stage1 F) => [newtm|]; rewrite Hinfer1 in Hinfer; try discriminate.
+  case Hinfer2 : (InferWidths_stage2 F newtm) => [nm|]; rewrite Hinfer2 in Hinfer; try discriminate.
+  inversion Hinfer; clear Hinfer.
+  rewrite H0 in Hinfer2; clear H0 nm H1 t.
+  case HF : F => [[v0 v1 pp ss]|f]; rewrite HF in Himplivm Hinfer1 Hinfer2; rewrite /InferWidths_stage2 in Hinfer2; try discriminate.
+  case Htransp : (InferWidths_transps pp newtm) => [nps|]; rewrite Htransp in Hinfer2; try discriminate.
+  case Htranss : (InferWidths_transss ss newtm) => [nss|]; rewrite Htranss in Hinfer2; try discriminate.
+  inversion Hinfer2; clear Hinfer2 H0 F' HF.
+  rewrite /make_vm_implicit in Himplivm.
+  case Himplips : (make_ps_implicit vm' (CEP.empty vertex_type) pp) => [vm''|]; rewrite Himplips in Himplivm; try discriminate.
+  intro Hps.
+  case Hps' : (ports_stmts_tmap nps nss vm') => [tmap|]; rewrite Hps' in Hps; try done.
+  assert (exists tmap', ports_stmts_tmap pp ss vm = Some tmap').
+  admit. (* 由 Hps' *)
+  destruct Hps as [vm0 [ct0 [Hports Hstmts]]].
+  destruct H as [tmap' Hps]; rewrite Hps.
+  generalize Htransp; apply InferWidths_trans_correct with (ss := ss) (nss := nss) (vm' := vm') (vm'' := vm'') (vm := vm) in Htransp; try done.
+  rewrite Hps in Htransp; inversion Htransp; clear Htransp; rewrite H0 in Hps; clear H0 tmap'; intro Htransp.
+  clear Hports Hstmts vm0 ct0 Hps' tmap. (* vm'全为expli，不包括任何前提 *)
+
+  (*InferWidths_transps pp newtm = Some nps -> InferWidths_transss ss newtm = Some nss ->
+  make_ps_implicit vm' (CEP.empty vertex_type) pp = Some vm'' -> make_ss_implicit vm' vm'' ss = Some vm -> ports_stmts_tmap pp ss vm = Some newtm *)
+
+  (* ports_stmts_tmap pp ss vm = Some tmap' -> type_of_ref pv tmap' = Some () -> 
+     code_type_find_vm_widths (type reg) pv vm = Some () *)
+
+
+  exists vm''; exists (CEP.empty def_expr). (* 不是empty，但先不check任何关于connection *)
+  split.
+  - admit.
+  - rewrite /InferWidths_stage1 in Hinfer1.
+    case Hps0 : (ports_stmts_tmap' pp ss) => [[tmap0 var2exprs]|]; rewrite Hps0 in Hinfer1; try discriminate.
+    case Hreg : (lsreg_stmts ss) => [lsreg|]; rewrite Hreg in Hinfer1; try discriminate.
+    case Hdraw : (drawg (CEP.elements var2exprs) tmap0 lsreg emptyg emptyg [::] [::]) => [[[[theg vertices] regg] reg_vertices]|]; rewrite Hdraw in Hinfer1; try discriminate.
+    case Htopo : (TopoSort.topo_sort vertices theg) => [inferorder||]; rewrite Htopo in Hinfer1; try discriminate.
+    case Htopo' : (TopoSort.topo_sort reg_vertices regg) => [t||]; rewrite Htopo' in Hinfer1; try discriminate; clear Htopo' t.
+    rewrite /ports_stmts_tmap in Hps. 
+    case Hpps : (ports_tmap pp vm) => [pmap|]; rewrite Hpps in Hps; try discriminate.
+    case Hpss : (stmts_tmap (pmap, pmap) ss vm) => [[tmap1 tmap2]|]; rewrite Hpss in Hps; try discriminate.
+    inversion Hps; clear Hps; rewrite H0 in Hpss; clear H0 tmap1.
+    clear Hpps.
+
+    specialize InferWidths_fun_correct with (pp := pp) (ss := ss) (inferorder := inferorder) (var2exprs := var2exprs) (tmap0 := tmap0) (newtm := newtm); intro Hinfer.
+    rewrite Hinfer1 Hps0 in Hinfer.
+    move : Hpss Himplivm Hinfer.
+    clear.
+    move : ss vm' vm pmap tmap2 vm'' newtm.
+    elim.
+    - simpl; intros; inversion Himplivm; apply CEP.Lemmas.Equal_refl.
+    - intros s st IH vm0 vm pmap tmap2 nvm newtm Hmaps Himplis Hinfer.
+      simpl; simpl in Hmaps; simpl in Himplis.
+      case Hmap : (stmt_tmap (pmap, pmap) s vm) => [[tmap' tmap2']|]; rewrite Hmap in Hmaps; try discriminate.
+      case Himpli : (make_s_implicit vm0 nvm s) => [vm'|]; rewrite Himpli in Himplis; try discriminate.
+      exists vm'; split.
+      - clear IH.
+        (*apply InferWidths_fun_correct with (pp := pp) (ss := (Qcons s st)) (hfs := s) in Hinfer1; try done.*)
+        specialize Hinfer with (hfs := s).
+        case Hs : s => [|r t|r reg|||r e|r e|r|c s1 s2]; rewrite Hs in Hmap Himpli Hinfer; simpl; try done.
+        - simpl in Hmap; simpl in Himpli; inversion Himpli; apply CEP.Lemmas.Equal_refl.
+        - (* reg *)
+          (*case Hrst : (reset reg) => [|rst_sig rst_val]; try done.
+          case Hft : (CEP.find r newtm) => [[ft ori]|].
+          - case Hval : (type_of_expr rst_val newtm) => [[ft_val p_val]|].
+            rewrite /connect_type; apply rwP with (P := ftype_equiv ft ft_val /\
+            check_connect_type
+              (list_gtypref (0%num, 0%num) ft HiF.Duplex)
+              (list_gtypref (0%num, 0%num) ft_val HiF.Duplex)). apply andP. split.
+            admit. (* cnct 要求 ftype_equiv *)
+            simpl in Hmap; simpl in Himpli.
+            case Hfindp : (CEP.find r pmap); rewrite Hfindp in Hmap; try discriminate.
+            destruct (type_of_expr (clock reg) pmap); try discriminate.
+            case Hft_vm : (code_type_find_vm_widths (type reg) r vm) => [[newt n]|]; rewrite Hft_vm in Hmap; try discriminate.
+            rewrite Hrst in Hmap.
+            case Hsig : (type_of_expr rst_sig pmap) => [[tf t]|]; rewrite Hsig in Hmap; try discriminate.
+            case Htf : tf => [f1||]; rewrite Htf in Hmap; try discriminate.
+            case Hf1 : f1 => [n1||||||]; rewrite Hf1 in Hmap; try discriminate.
+            - (* Fuint1 rst *) 
+              case Hn1 : n1 => [|n0]; rewrite Hn1 in Hmap; try discriminate.
+              destruct n0; try discriminate; clear Hsig Htf Hf1 Hn1 n1 f1 t tf.
+              assert (exists ft_val', type_of_expr rst_val (CEP.add r (newt, HiF.Duplex) pmap) = Some ft_val').
+              admit.
+              destruct H as [[ft_val' p_val'] Hval']; rewrite Hval' in Hmap; clear Hval' ft_val' p_val'.
+              inversion Hmap; clear Hmap.
+              assert (CEP.find r tmap = CEP.find r tmap').
+              admit. (* s = Sreg r reg 不在 st 中，由Hmaps *)
+              rewrite H -H0 in Hft; clear H Hmaps H1 H0 f Hfindp.
+              rewrite CEP.Lemmas.find_add_eq in Hft; try apply PVM.SE.eq_refl.
+              inversion Hft; clear Hft; rewrite H0 in Hft_vm; clear H0 H1 ori newt.
+              admit.
+            - (* aync *)
+              clear Hsig Htf Hf1 f1 t tf.
+              assert (exists ft_val', type_of_expr rst_val pmap = Some ft_val').
+              admit.
+              destruct H as [[ft_val' p_val'] Hval']; rewrite Hval' in Hmap; clear Hval' ft_val' p_val'.
+              inversion Hmap; clear Hmap.
+              assert (CEP.find r tmap = CEP.find r tmap').
+              admit. (* s = Sreg r reg 不在 st 中，由Hmaps *)
+              rewrite H -H0 in Hft; clear H Hmaps H1 H0 f Hfindp.
+              rewrite CEP.Lemmas.find_add_eq in Hft; try apply PVM.SE.eq_refl.
+              inversion Hft; clear Hft; rewrite H0 in Hft_vm; clear H0 H1 ori newt.
+              admit. (* TBD *)
+          - admit. (* None则有错 *)
+          - admit. (* None则有错 *)*)
+          admit.
+        - (* cnct *)
+          case Hr : r => [ref|||]; rewrite Hr in Hs Hinfer.
+          case He : e => [t c| c e1 | u e1 | op e1 e2 | c e1 e2 | c e1 | r2 ]; rewrite He in Hs Hinfer.
+          - (* expr *)
+          1,2,3,4,5,6 : rewrite -He; rewrite -He in Hinfer; clear He Hs Hr.
+          1,2,3,4,5,6 : case Hreft : (type_of_ref ref newtm) => [[t_tgt ori]|]; rewrite Hreft in Hinfer.
+          1,3,5,7,9,11 : case Hexprt : (type_of_expr e newtm) => [[t_expr p_expr]|]; rewrite Hexprt in Hinfer.
+          1,3,5,7,9,11 : apply Hinfer; try done.
+          admit. (* Qin_cons *)
+          admit. (* Hypo *)
+          admit. (* Qin_cons *)
+          admit. (* Hypo *)
+          admit. (* Qin_cons *)
+          admit. (* Hypo *)
+          admit. (* Qin_cons *)
+          admit. (* Hypo *)
+          admit. (* Qin_cons *)
+          admit. (* Hypo *)
+          admit. (* Qin_cons *)
+          admit. (* Hypo *)
+          admit. (* None则有错 *)
+          admit. (* None则有错 *)
+          admit. (* None则有错 *)
+          admit. (* None则有错 *)
+          admit. (* None则有错 *)
+          admit. (* None则有错 *)
+          admit. (* None则有错 *)
+          admit. (* None则有错 *)
+          admit. (* None则有错 *)
+          admit. (* None则有错 *)
+          admit. (* None则有错 *)
+          admit. (* None则有错 *)
+          - (* ref *)
+          case Hr2 : r2 => [ref_src|||]; rewrite Hr2 in Hinfer.
+          case Hreft : (type_of_ref ref newtm) => [[t_tgt ori]|]; rewrite Hreft in Hinfer.
+          case Hexprt : (type_of_ref ref_src newtm) => [[t_expr p_expr]|]; rewrite Hexprt in Hinfer; try done.
+          apply Hinfer; try done.
+          admit. (* Qin_cons *)
+          admit. (* Hypo *)
+          admit. (* None则有错 *)
+          admit. (* None则有错 *)
+          admit. (* no subfield *)
+          admit. (* no subindex *)
+          admit. (* no subaccess *)
+          admit. (* no subfield *)
+          admit. (* no subindex *)
+          admit. (* no subaccess *)
+        - (* when *)
+          admit.
+      - apply IH with (vm' := vm0) (pmap := tmap') (tmap2 := tmap2); try done.
+        admit.
+        intros.
+        apply Hinfer with (hfs := hfs) in H; try done.
 Admitted.
 
 Definition type_of_vx (x : vertex_type) : fgtyp :=
@@ -1043,11 +1477,188 @@ Definition vm_le (vm : CEP.t vertex_type) (vm' : CEP.t vertex_type) : Prop :=
   | _, _ => false
   end.
 
+Lemma InferWidths_trans_correct' : forall v vm' t' F' mv ps ss newtm ft ori, CEP.find v vm' = Some t' -> Sem F' vm' -> InferWidths_stage2 (FInmod mv ps ss) newtm = Some F' ->
+  type_of_ref v newtm = Some (ft, ori) -> ft = (Gtyp (type_of_vx t')).
+Proof.
+Admitted.
+
+Lemma geq_conj2mux : forall tmap (gt initt : fgtyp) (el : seq HiFP.hfexpr) eftl (nt : fgtyp), (forall (texpr : HiFP.hfexpr) (te : fgtyp) (p : ftype_not_implicit_width (Gtyp te)), texpr \in el -> type_of_expr texpr tmap = Some (exist ftype_not_implicit_width (Gtyp te) p) -> ((sizeof_fgtyp gt) >= (sizeof_fgtyp te))) ->
+  fil_ftlist [seq type_of_expr e tmap | e <- el] = Some eftl -> sizeof_fgtyp initt = 0 -> max_ftlist eftl initt = Some nt -> ((sizeof_fgtyp gt) >= (sizeof_fgtyp nt)).
+Proof.
+Admitted.
+
+Fixpoint find_sub_expr4v (pv : ProdVarOrder.t) (lhsl : seq (ProdVarOrder.t * fgtyp * HiF.forient)) (rstl : seq HiFP.hfexpr) : option (seq HiFP.hfexpr) :=
+  match lhsl, rstl with
+  | nil, nil => Some nil
+  | (hd, _, _) :: tl, hde :: tle => if (hd == pv) then Some [:: hde]
+                              else find_sub_expr4v pv tl tle
+  | _, _ => None
+  end.
+
+Fixpoint find_sub_non_passive4v (pv : ProdVarOrder.t) (lhsl rhsl : seq (ProdVarOrder.t * fgtyp * HiF.forient)) : option (seq HiFP.hfexpr) :=
+  match lhsl, rhsl with
+  | nil, nil => Some nil
+  | (hd, _, HiF.Duplex) :: tl, (hde, _, HiF.Source) :: tle 
+  | (hd, _, HiF.Sink) :: tl, (hde, _, HiF.Source) :: tle 
+  | (hd, _, HiF.Sink) :: tl, (hde, _, HiF.Duplex) :: tle 
+  | (hd, _, HiF.Duplex) :: tl, (hde, _, HiF.Duplex) :: tle => if (hd == pv) then Some [:: (Eref (Eid hde))]
+                                                            else find_sub_non_passive4v pv tl tle
+  | (hd, _, HiF.Source) :: tl, (hde, _, HiF.Sink) :: tle 
+  | (hd, _, HiF.Source) :: tl, (hde, _, HiF.Duplex) :: tle 
+  | (hd, _, HiF.Duplex) :: tl, (hde, _, HiF.Sink) :: tle => if (hde == pv) then Some [:: (Eref (Eid hd))]
+                                                            else find_sub_non_passive4v pv tl tle
+  | _, _ => None
+  end.
+
+Fixpoint find_sub_expr (pv : ProdVarOrder.t) (s : HiFP.hfstmt) (tmap : CEP.t (ftype * HiF.forient)) : option (seq HiFP.hfexpr) :=
+  match s with
+  | Sreg v r => match reset r with
+                | NRst => Some nil
+                | Rst _ rst_val => match list_gtypexpr rst_val (type r), list_gtypref v (type r) HiF.Duplex with
+                                  | Some rstl, lhsl => find_sub_expr4v pv lhsl rstl
+                                  | _, _ => None
+                                  end
+                end
+  | Snode v e => match type_of_expr e tmap with
+                | Some (exist t _) => match list_gtypexpr e t, list_gtypref v t HiF.Sink with
+                            | Some rstl, lhsl => find_sub_expr4v pv lhsl rstl
+                            | _, _ => None
+                            end
+                | _ => None
+                end
+  | Sfcnct (Eid ref_tgt) (Eref (Eid ref_src)) =>
+                match type_of_ref ref_tgt tmap, type_of_ref ref_src tmap with
+                | Some (t_tgt, ori_tgt), Some (t_src, ori_src) =>
+                            match list_gtypref ref_tgt t_tgt ori_tgt, list_gtypref ref_src t_src ori_src with
+                            | lhsl, rhsl => find_sub_non_passive4v pv lhsl rhsl
+                            end
+                | _, _ => None
+                end
+  | Sfcnct (Eid ref_tgt) (Eref _) => None
+  | Sfcnct (Eid ref_tgt) expr_src =>
+                match type_of_ref ref_tgt tmap, type_of_expr expr_src tmap with
+                | Some (t_tgt, ori_tgt), Some (exist t_src _) =>
+                      match list_gtypexpr expr_src t_src, list_gtypref ref_tgt t_tgt ori_tgt with
+                      | Some rstl, lhsl => find_sub_expr4v pv lhsl rstl
+                      | _, _ => None
+                      end
+                | _, _ => None
+                end
+  | Swhen _ s1 s2 => match find_sub_exprs pv s1 tmap, find_sub_exprs pv s2 tmap with
+                    | Some e1, Some e2 => Some (e1 ++ e2)
+                    | _,_ => None
+                    end
+  | _ => Some nil
+  end
+with find_sub_exprs (v : ProdVarOrder.t) (ss : HiFP.hfstmt_seq) (tmap : CEP.t (ftype *HiF.forient)) : option (seq HiFP.hfexpr) :=
+  match ss with
+  | Qnil => Some nil
+  | Qcons s ss' => match find_sub_expr v s tmap, find_sub_exprs v ss' tmap with
+                  | Some e, Some el => Some (e ++ el)
+                  | _, _ => None
+                  end
+  end.
+
+Lemma Sem_wdgeqmax ss : forall vm_old vm_new tmap, Sem_frag_stmts vm_old ss vm_new tmap -> (forall v t el, CEP.find v vm_new = Some t -> 
+  find_sub_exprs v ss tmap = Some el -> (forall e te (p : ftype_not_implicit_width (Gtyp te)), e \in el -> type_of_expr e tmap = Some (exist ftype_not_implicit_width (Gtyp te) p) -> sizeof_fgtyp (type_of_vx t) >= sizeof_fgtyp te)).
+Proof.
+Admitted.
+
+Lemma Semgeqinfer : forall pp ss mv vm tmap newtm, Sem (FInmod mv pp ss) vm -> ports_stmts_tmap pp ss vm = Some tmap -> InferWidths_stage1 (FInmod mv pp ss) = Some newtm -> (forall e t0 t1 (p0 : ftype_not_implicit_width (Gtyp t0)) (p1 : ftype_not_implicit_width (Gtyp t1)), type_of_expr e tmap = Some (exist ftype_not_implicit_width (Gtyp t0) p0) -> type_of_expr e newtm = Some (exist ftype_not_implicit_width (Gtyp t1) p1) -> sizeof_fgtyp t0 >= sizeof_fgtyp t1).
+Proof.
+Admitted.
+
+Lemma find_sub_exprs_correct : forall v ps ss tmap var2exprs, ports_stmts_tmap' ps ss = Some (tmap, var2exprs) -> CEP.find v var2exprs = find_sub_exprs v ss tmap.
+Proof.
+Admitted.
+
+Lemma set_find_sub : forall checkt nt nt0 n ori ori_v initt, ft_find_sub checkt n ori_v = Some (Gtyp initt, ori) -> ft_set_sub checkt nt n = Some nt0 -> ft_find_sub nt0 n ori_v = Some (Gtyp nt, ori)
+with set_find_sub_f : forall checkf nf nf0 n ori ori_v initt, ft_find_sub_f checkf n ori_v = Some (Gtyp initt, ori) -> ft_set_sub_f checkf nf n = Some nf0 -> ft_find_sub_f nf0 n ori_v = Some (Gtyp nf, ori).
+Proof.
+Admitted.
+
 Theorem InferWidths_correct' :
-  forall (F : HiFP.hfmodule) (vm : CEP.t vertex_type) (vm' : CEP.t vertex_type) (ct : CEP.t def_expr),
+  forall (F : HiFP.hfmodule) (vm : CEP.t vertex_type) (vm' : CEP.t vertex_type),
     match InferWidths_m F with
-    | Some (F', _) => Sem F' vm' ct -> Sem F vm ct -> vm_le vm vm'
+    | Some (F', _) => Sem F' vm' -> Sem F vm -> vm_le vm vm'
     | _ => True
     end.
 Proof.
+  intros F vm vm'.
+  case Hinfer : (InferWidths_m F) => [[F' newtm]|]; try done.
+  intros Hsem' Hsem.
+  rewrite /vm_le; intro v.
+  case Ht' : (CEP.find v vm') => [t'|].
+  case Ht : (CEP.find v vm) => [t|]; try done.
+  case Himpli : (not_implicit (type_of_vx t')); try done.
+  rewrite /InferWidths_m in Hinfer.
+  case Hinfer1 : (InferWidths_stage1 F) => [newtm'|]; rewrite Hinfer1 in Hinfer; try discriminate.
+  case Hinfer2 : (InferWidths_stage2 F newtm') => [nm|]; rewrite Hinfer2 in Hinfer; try discriminate.
+  inversion Hinfer; clear Hinfer; rewrite H0 in Hinfer2; clear H0 nm; rewrite H1 in Hinfer1 Hinfer2; clear H1 newtm'.
+  generalize Hinfer1; rewrite /InferWidths_stage1 in Hinfer1; intros Hstage1.
+  case HF : F => [mv ps ss|]; rewrite HF in Hinfer1 Hstage1; try discriminate.
+  rewrite HF in Hsem Hinfer2; clear HF F.
+  case Hpre : (ports_stmts_tmap' ps ss) => [[tmap' var2exprs]|]; rewrite Hpre in Hinfer1; try discriminate.
+  case Hrl : (lsreg_stmts ss) => [rl|]; rewrite Hrl in Hinfer1; try discriminate.
+  case Hdraw : (drawg (CEP.elements var2exprs) tmap' rl emptyg emptyg [::] [::]) => [[[[theg vertices]regg] reg_vertices]|]; rewrite Hdraw in Hinfer1; try discriminate.
+  case Htopo : (TopoSort.topo_sort vertices theg) => [inferorder||]; rewrite Htopo in Hinfer1; try discriminate.
+  destruct (TopoSort.topo_sort reg_vertices regg); try discriminate; clear l.
+
+  assert (v \in inferorder).
+  admit. (* inferorder 的正确性，是展开时的标号 *)
+  assert (exists order1 order2, inferorder = order1 ++ (v :: order2) /\ ~ v \in order1 /\ ~ v \in order2).
+  admit. (* 由H推出 *)
+  clear H.
+  move : H0 => [order1 [order2 [H2 [Horder1 Horder2]]]].
+  rewrite H2 in Hinfer1; rewrite /InferWidths_fun in Hinfer1.
+  case Hinfer1' : (InferWidths_fun order1 var2exprs tmap') => [tmap0|].
+  assert (Hinfer2' : InferWidths_fun (v :: order2) var2exprs tmap0 = Some newtm).
+  move : Hinfer1 Hinfer1'.
+  apply infer_cons_order.
+  clear Hinfer1 Hdraw Htopo theg vertices regg reg_vertices.
+  generalize Hinfer2'; simpl in Hinfer2'; intros Hod2.
+  case Hel : (CEP.find v var2exprs) => [el|]; rewrite Hel in Hinfer2'; try discriminate.
+  case Hinfer1 : (InferWidth_fun v el tmap0) => [newtm'|]; rewrite Hinfer1 in Hinfer2'; try discriminate.
+  rewrite /InferWidth_fun in Hinfer1.
+  case Hfil : (fil_ftlist [seq type_of_expr e tmap0 | e <- el]) => [eftl|]; rewrite Hfil in Hinfer1; try done.
+  case Hinit : (CEP.find (v.1, 0%num) tmap0) => [[init ori_v]|]; rewrite Hinit in Hinfer1; try discriminate.
+  case Hf : (ft_find_sub init v.2 ori_v) => [[f ori]|]; rewrite Hf in Hinfer1; try discriminate.
+  case Hinitt : f => [initt||]; rewrite Hinitt in Hinfer1; try discriminate.
+  rewrite Hinitt in Hf; clear Hinitt f.
+  assert (Himpli' : not_implicit initt = false). 
+  admit. (* drawg只考虑implicit *)
+  case Hmax : (max_ftlist eftl initt) => [nt|]; rewrite Hmax in Hinfer1; try discriminate.
+  case Hset : (ft_set_sub init nt v.2) => [nt0|]; rewrite Hset in Hinfer1; try discriminate. 
+  inversion Hinfer1; clear Hinfer1.
+  apply InferWidths_trans_correct' with (F' := F') (mv := mv) (ps := ps) (ss := ss) (newtm := newtm) (ft := Gtyp nt) (ori := ori) in Ht'; try done.
+  inversion Ht'; clear Ht'; rewrite -H1; clear H1.
+  generalize Hsem; rewrite /Sem in Hsem.
+  case Hpre0 : (ports_stmts_tmap ps ss vm) => [tmap0'|]; rewrite Hpre0 in Hsem; try done.
+  destruct Hsem as [vm0 [ct0 [_ Hsems]]]; intro Hsem.
+  apply geq_conj2mux with (tmap := tmap0) (initt := initt) (el := el) (eftl := eftl); try done.
+  intros.
+  assert (Hte : exists t0 p0, type_of_expr texpr tmap0' = Some (exist ftype_not_implicit_width (Gtyp t0) p0)).
+  admit. (* tl中应全为gtyp expr *)
+  destruct Hte as [t0 [p0 Hte]].
+  apply Semgeqinfer with (tmap := tmap0') (newtm := newtm) (e := texpr) (t0 := t0) (t1 := te) (p0 := p0) (p1 := p) in Hsem; try done.
+  apply Sem_wdgeqmax with (v := v) (t := t) (el := el) (e := texpr) (te := t0) (p := p0) in Hsems; try done.
+  move : Hsem Hsems; apply leq_trans.
+  generalize Hpre; apply find_sub_exprs_correct with (v := v) in Hpre; try done; rewrite -Hel Hpre.
+  move : Hpre0.
+  admit.
+  move : H1 Hod2.
+  admit. (* infer后面的部分不影响expr的type *)
+  admit.
+  assert (type_of_ref v newtm = type_of_ref v newtm').
+  move : Horder2 Hinfer2'.
+  admit.
+  rewrite H /type_of_ref -H0 CEP.Lemmas.find_add_eq; clear H; try apply PVM.SE.eq_refl. 
+  move : Hf Hset.
+  apply set_find_sub.
+
+  admit. (* None则有错 *)
+  admit. (* None则有错 *)
+  case Ht : (CEP.find v vm); try done.
 Admitted.
+
+Search (type_of_ref).
